abp/generated/abp/FairMediumStates.thy
@@ -3,7 +3,7 @@
  * This file was generated from FairMedium.maa and will be overridden when changed. To change
  * permanently, consider changing the model itself.
  *
- * Generated on Oct 12, 2018 1:15:31 PM by isartransformer 2.0.0
+ * Generated on Oct 16, 2018 10:17:27 PM by isartransformer 3.1.0
  *)
 theory FairMediumStates
   imports MediumDatatype
@@ -15,14 +15,14 @@ begin
 datatype FairMediumSubstate = Single
 
 (* And these have also the variables *)
-datatype FairMediumState = FairMediumState FairMediumSubstate (* counter = *) "nat"
+datatype FairMediumState = FairMediumState FairMediumSubstate (* counter = *) "int"
 
 (* Function to get the substate *)
 fun getFairMediumSubState :: "FairMediumState \<Rightarrow> FairMediumSubstate" where
     "getFairMediumSubState (FairMediumState s _) = s"
 
 (* Functions to get the variables *)
-fun getCounter :: "FairMediumState \<Rightarrow> nat" where
+fun getCounter :: "FairMediumState \<Rightarrow> int" where
 "getCounter (FairMediumState _ var_counter) = var_counter"
 
 
