abp/generated/abp/MediumStates.thy
@@ -3,7 +3,7 @@
  * This file was generated from Medium.maa and will be overridden when changed. To change
  * permanently, consider changing the model itself.
  *
- * Generated on Oct 12, 2018 1:15:32 PM by isartransformer 2.0.0
+ * Generated on Oct 16, 2018 10:17:27 PM by isartransformer 3.1.0
  *)
 theory MediumStates
   imports MediumDatatype
@@ -15,14 +15,14 @@ begin
 datatype MediumSubstate = Single
 
 (* And these have also the variables *)
-datatype MediumState = MediumState MediumSubstate (* coin = *) "nat"
+datatype MediumState = MediumState MediumSubstate (* coin = *) "int"
 
 (* Function to get the substate *)
 fun getMediumSubState :: "MediumState \<Rightarrow> MediumSubstate" where
     "getMediumSubState (MediumState s _) = s"
 
 (* Functions to get the variables *)
-fun getCoin :: "MediumState \<Rightarrow> nat" where
+fun getCoin :: "MediumState \<Rightarrow> int" where
 "getCoin (MediumState _ var_coin) = var_coin"
 
 
